books/kestrel/crypto/r1cs/tools/axe-syntax-functions-r1cs.lisp
@@ -1,0 +1,44 @@
+; Syntactic functions for Axe R1CS prover
+;
+; Copyright (C) 2020 Kestrel Institute
+;
+; License: A 3-clause BSD license. See the file books/3BSD-mod.txt.
+;
+; Author: Eric Smith (eric.smith@kestrel.edu)
+
+;;;;;;;;;;;;;;;;;;;;;;;;;;;;;;;;;;;;;;;;;;;;;;;;;;;;;;;;;;;;;;;;;;;;;;;;;;;;;;;;
+
+(in-package "R1CS")
+
+(include-book "../portcullis")
+(include-book "kestrel/axe/dag-arrays" :dir :system)
+
+(defun acl2::var-less-than-unquoted-keyp (var-darg key-darg acl2::dag-array)
+  (declare (xargs :guard (and (or (acl2::myquotep var-darg)
+                                  (and (natp var-darg)
+                                       (acl2::pseudo-dag-arrayp 'acl2::dag-array acl2::dag-array (+ 1 var-darg))))
+                              (or (acl2::myquotep key-darg)
+                                  (and (natp key-darg)
+                                       (acl2::pseudo-dag-arrayp 'acl2::dag-array acl2::dag-array (+ 1 key-darg)))))))
+  (and (consp key-darg) ;checks for quotep
+       (let ((unquoted-key (unquote key-darg)))
+         (and (symbolp unquoted-key)
+              (natp var-darg)
+              (let ((var-expr (aref1 'acl2::dag-array acl2::dag-array var-darg)))
+                (and (symbolp var-expr)
+                     (symbol-< var-expr unquoted-key)))))))
+
+(defun acl2::var-not-less-than-unquoted-keyp (var-darg key-darg acl2::dag-array)
+  (declare (xargs :guard (and (or (acl2::myquotep var-darg)
+                                  (and (natp var-darg)
+                                       (acl2::pseudo-dag-arrayp 'acl2::dag-array acl2::dag-array (+ 1 var-darg))))
+                              (or (acl2::myquotep key-darg)
+                                  (and (natp key-darg)
+                                       (acl2::pseudo-dag-arrayp 'acl2::dag-array acl2::dag-array (+ 1 key-darg)))))))
+  (and (consp key-darg) ;checks for quotep
+       (let ((unquoted-key (unquote key-darg)))
+         (and (symbolp unquoted-key)
+              (natp var-darg)
+              (let ((var-expr (aref1 'acl2::dag-array acl2::dag-array var-darg)))
+                (and (symbolp var-expr)
+                     (not (symbol-< var-expr unquoted-key))))))))
